

Context Free Languages: Expressionally μ -regular expressions

Zoe Stafford

October 30, 2025

Outline

Motivation

μ -Regular Expressions

Fixed points

Fixed points of μ -Regular Expressions

Motivation

- ▶ Classify sets of words (*languages*)
- ▶ Show language membership is computable/efficient
- ▶ Describe languages

Motivation

- ▶ Regular expressions 😇

$$0x[0-9, a-f][0-9, a-f]^* + [1-9][0-9]^*$$

- ▶ Context Free Grammars 😬

$$S \rightarrow H \mid D$$

$$A \rightarrow 0 \mid 1 \mid \dots \mid f$$

$$H' \rightarrow AH' \mid \epsilon$$

$$H \rightarrow 0xAH'$$

$$B \rightarrow 0 \mid 1 \mid \dots \mid 9$$

$$B' \rightarrow 1 \mid 1 \mid \dots \mid 9$$

$$D' \rightarrow BD' \mid \epsilon$$

$$D \rightarrow B'D'$$

Notation

- ▶ S^* is set of finite *words* on S — ie finite sequences of elements in S
- ▶ ϵ : empty word
- ▶ uv : concatenation of u and v
- ▶ letters: $x, y, z \in \Sigma$
- ▶ words: $u, v, w \in \Sigma^*$
- ▶ regular expressions: A, B, C
- ▶ Variables: X, Y, Z

Regular Expressions

Define set R_Σ of regular expressions over Σ inductively:

$$\begin{array}{c} \frac{}{\emptyset \in R_\Sigma} \qquad \frac{}{\epsilon \in R_\Sigma} \qquad \frac{x \in \Sigma}{x \in R_\Sigma} \qquad \frac{A \in R_\Sigma \quad B \in R_\Sigma}{AB \in R_\Sigma} \\[2ex] \frac{A \in R_\Sigma \quad B \in R_\Sigma}{A + B \in R_\Sigma} \qquad \frac{A \in R_\Sigma}{A^* \in R_\Sigma} \end{array}$$

Regular Expressions

Example

$$0 + 1(0 + 1)^*00$$

Regular Expressions

Example

$$0 + 1(0 + 1)^*00$$

Multiples of 4 (in binary)

Regular Expressions

Semantics

- ▶ Consider $A \in R_\Sigma$
- ▶ We define the *language* of A : $L(A) \subseteq \Sigma^*$

Regular Expressions

Semantics

- ▶ Consider $A \in R_\Sigma$
- ▶ We define the *language* of A : $L(A) \subseteq \Sigma^*$
- ▶ By induction!

Regular Expressions

Semantics

- ▶ $L(x) = \{x\}$ for $x \in \Sigma$
- ▶ $L(\epsilon) = \{\epsilon\}$
- ▶ $L(\emptyset) = \emptyset$
- ▶ $L(AB) = L(A)L(B) = \{uv \mid u \in L(A), v \in L(B)\}$
- ▶ $L(A + B) = L(A) \cup L(B)$
- ▶ $L(A^*) = \{u_1 \dots u_n \mid n \in \mathbb{N}, u_1, \dots, u_n \in L(A)\}$

Regular Expressions

Not an Example — Balanced Brackets

$$L_1 := \{ \langle \rangle, \langle \rangle \langle \rangle, \langle \langle \rangle \rangle, \langle \langle \rangle \rangle \langle \rangle, \langle \rangle \langle \rangle \langle \rangle, \dots \}$$

Regular Expressions

Not an Example — Balanced Brackets

$$L_1 := \{ \langle \rangle, \langle \rangle \langle \rangle, \langle \langle \rangle \rangle, \langle \langle \rangle \rangle \langle \rangle, \langle \rangle \langle \rangle \langle \rangle, \dots \}$$

Want $A \in R_{\{\langle, \rangle\}}$ that denotes L_1 :

- Each $w \in L_1$ is some of form $\langle u_1 \rangle \langle u_2 \rangle \dots \langle u_n \rangle$ for $u_i \in L_1$

Regular Expressions

Not an Example — Balanced Brackets

$$L_1 := \{ \langle \rangle, \langle \rangle \langle \rangle, \langle \langle \rangle \rangle, \langle \langle \rangle \rangle \langle \rangle, \langle \rangle \langle \rangle \langle \rangle, \dots \}$$

Want $A \in R_{\{\langle, \rangle\}}$ that denotes L_1 :

- ▶ Each $w \in L_1$ is some of form $\langle u_1 \rangle \langle u_2 \rangle \dots \langle u_n \rangle$ for $u_i \in L_1$
- ▶ $A = (\langle B \rangle)^*$ for some B
- ▶ B denotes balanced brackets

Regular Expressions

Not an Example — Balanced Brackets

$$L_1 := \{ \langle \rangle, \langle \rangle \langle \rangle, \langle \langle \rangle \rangle, \langle \langle \rangle \rangle \langle \rangle, \langle \rangle \langle \rangle \langle \rangle, \dots \}$$

Want $A \in R_{\{\langle, \rangle\}}$ that denotes L_1 :

- ▶ Each $w \in L_1$ is some of form $\langle u_1 \rangle \langle u_2 \rangle \dots \langle u_n \rangle$ for $u_i \in L_1$
- ▶ $A = (\langle B \rangle)^*$ for some B
- ▶ B denotes balanced brackets
- ▶ So $B = A$
- ▶ $A = (\langle A \rangle)^*$ 😱

μ -Regular Expressions

- ▶ Recursion!
- ▶ Set of variables \mathcal{V}

$$\frac{X \in \mathcal{V}}{X \in R_\Sigma}$$

$$\frac{X \in \mathcal{V} \quad A \in R_\Sigma}{\mu X. A \in R_\Sigma}$$

μ -Regular Expressions

Example

$$\mu S.(\langle S \rangle)^*$$

μ -Regular Expressions

Example

$$\mu S.(\langle S \rangle)^*$$

Balanced brackets 🤖

μ -Regular Expressions

Example

$$\mu S.(\langle S \rangle)^*$$

Balanced brackets 🤖

$$\mu E.[1 - 9][0 - 9]^* + (E - E) + (E \times E) + (E \div E)$$

μ -Regular Expressions

Example

$$\mu S.(\langle S \rangle)^*$$

Balanced brackets 🤖

$$\mu E.[1 - 9][0 - 9]^* + (E - E) + (E \times E) + (E \div E)$$

Arithmetic

μ -Regular Expressions

Recursion

$$\mu X.A$$

- ▶ A 'is' a function of X
- ▶ $\mu X.A$ finds *fixed point* of A (w.r.t. X)

$$\mu X.A \equiv A[X \mapsto \mu X.A]$$

μ -Regular Expressions

Recursion

$$\mu X.A$$

- ▶ A 'is' a function of X
- ▶ $\mu X.A$ finds *fixed point* of A (w.r.t. X)

$$\mu X.A \equiv A[X \mapsto \mu X.A]$$

- ▶ e.g. $\mu X.\epsilon + \langle X \rangle \equiv \epsilon + \langle (\mu X.\epsilon + \langle X \rangle) \rangle$

μ -Regular Expressions

Example

$$A^* \equiv \epsilon + AA^*$$

μ -Regular Expressions

Example

$$A^* \equiv \epsilon + AA^*$$

- Let $A^* := \mu X. \epsilon + AX$ (for some *fresh* X)

$$\begin{aligned} A^* &= \mu X. \epsilon + AX \\ &\equiv \epsilon + A(\mu X. \epsilon + AX) \\ &= \epsilon + AA^* \end{aligned}$$

μ -Regular Expressions

Variable binding

- ▶ Assumption: variable names are unique
 - ▶ Bad: $\mu X.\mu X.X$
 - ▶ Good: $\mu X.\mu Y.X$

μ -Regular Expressions

Variable binding

- ▶ Assumption: variable names are unique
 - ▶ Bad: $\mu X.\mu X.X$
 - ▶ Good: $\mu X.\mu Y.X$
- ▶ $FV(A)$ = free variables of A :

μ -Regular Expressions

Variable binding

- ▶ Assumption: variable names are unique
 - ▶ Bad: $\mu X.\mu X.X$
 - ▶ Good: $\mu X.\mu Y.X$
- ▶ $\text{FV}(A)$ = free variables of A :

$$\text{FV}(X) = \{X\} \quad (X \in \mathcal{V})$$

$$\text{FV}(\mu X.A) = \text{FV}(A) \setminus \{X\}$$

$$\text{FV}(AB) = \text{FV}(A) \cup \text{FV}(B)$$

$$\text{FV}(A + B) = \text{FV}(A) \cup \text{FV}(B)$$

$$\text{FV}(\epsilon) = \text{FV}(\emptyset) = \text{FV}(x) = \emptyset \quad (x \in \Sigma)$$

μ -Regular Expressions

Semantics

- For $X \in \mathcal{V}$, $L(X) = \dots$

μ -Regular Expressions

Semantics

- ▶ For $X \in \mathcal{V}$, $L(X) = \dots$
- ▶ Add *context*: map $\sigma : \text{FV}(A) \rightarrow \Sigma^*$
- ▶ $L^\sigma(X) = \sigma(X)$

μ -Regular Expressions

Semantics

- ▶ For $X \in \mathcal{V}$, $L(X) = \dots$
- ▶ Add *context*: map $\sigma : \text{FV}(A) \rightarrow \Sigma^*$
- ▶ $L^\sigma(X) = \sigma(X)$
- ▶ $L^\sigma(A + B) = L^\sigma(A) \cup L^\sigma(B)$
- ▶ $L^\sigma(AB) = L^\sigma(A)L^\sigma(B)$

μ -Regular Expressions

- ▶ $L^\sigma(\mu X.A) = \dots$
- ▶ $L^\sigma(A)$?? No: σ not defined on X 😱

μ -Regular Expressions

- ▶ $L^\sigma(\mu X.A) = \dots$
- ▶ $L^\sigma(A)$?? No: σ not defined on X 😱

$$f_A(M) := L^{\sigma \cup \{X \mapsto M\}}(A)$$

μ -Regular Expressions

- ▶ $L^\sigma(\mu X.A) = \dots$
- ▶ $L^\sigma(A)$?? No: σ not defined on X 😱

$$f_A(M) := L^{\sigma \cup \{X \mapsto M\}}(A)$$

- ▶ Fixed point of f_A : N such that $f_A(N) = N$
- ▶ Does fixed point exist? 🤔
- ▶ Which one do we pick? 🤔

μ -Regular Expressions

- ▶ $L^\sigma(\mu X.A) = \dots$
- ▶ $L^\sigma(A)$?? No: σ not defined on X 😱

$$f_A(M) := L^{\sigma \cup \{X \mapsto M\}}(A)$$

- ▶ Fixed point of f_A : N such that $f_A(N) = N$
- ▶ Does fixed point exist? 🤔
- ▶ Which one do we pick? 🤔
- ▶ Pick the *least fixed point*

Fixed points

- ▶ The *least fixed point* of f is minimum element of

$$\{N \mid f(N) = N\}$$

- ▶ Written $\mu(f)$ or $\mu(x \mapsto f(x))$
- ▶ Kleene fixed point theorem describes least fixed point

Fixed points

Notation

- ▶ For function $f : A \rightarrow B$ and subset $D \subseteq A$, the image of D is

$$f[D] := \{f(x) \mid x \in D\}$$

- ▶ For partial order D and subset $A \subseteq D$, an *upper bound* of A is an $x \in D$ with $\forall y \in A. y \leq x$
- ▶ The *supremum* $\sup A$ is the least upper bound of A
 - ▶ Not defined for all A !

$$f^n(x) = \underbrace{f(f(\dots f(n) \dots))}_{n \text{ times}}$$

Fixed points

Partial orders

- ▶ Let \leq be a partial order on D
- ▶ A *directed subset* of D is non-empty subset $E \subseteq D$ s.t. every $a, b \in E$ have an upper bound $c \in E$ with $a \leq c$ and $b \leq c$
- ▶ D is a *directed-complete partial order* (*dcpo*) when every directed subset of D has a supremum (least upper bound)

Fixed points

Scott-continuity

- ▶ Let D be partial order
- ▶ Function $f : D \rightarrow D$ is *Scott-continuous* when f preserves directed supremums
- ▶ ie for any directed subset A of D , $f(\sup D) = \sup(f[D])$

Fixed points

Kleene fixed point theorem

- ▶ Let D be dcpo with least element \perp
- ▶ Let $f : D \rightarrow D$ be Scott-continuous
- ▶ Then the least fixed point of f is $\sup\{\perp, f(\perp), f(f(\perp)), \dots\}$

Fixed points

Kleene fixed point theorem - proof

- ▶ Let $M = \{f^n(\perp) \mid n \in \mathbb{N}\}$
- ▶ $\sup M$ exists since M is directed subset
- ▶ Need to show:
 1. $\sup M$ is a fixed point
 2. $\sup M$ is the least fixed point

Fixed points

Kleene fixed point theorem - proof (1)

$$\begin{aligned} f(\sup M) &= \sup(f[M]) \\ &= \sup\{f^n(\perp) \mid n \in \mathbb{N}, n \geq 1\} \\ &= \sup(M \setminus \{\perp\}) \\ &= \sup M \end{aligned}$$

Fixed points

Kleene fixed point theorem - proof (2)

- ▶ For any fixed point N of f , we need $\sup M \leq N$
- ▶ Claim: $f^n(\perp) \leq N$ for all n — proof by induction:
- ▶ case $n = 0$: $f^0(\perp) = \perp \leq N$
- ▶ case $n = k + 1$:
 - ▶ by IH $f^k(\perp) \leq N$
 - ▶ Lemma: f is monotonic
 - ▶ So $f^{k+1} \leq f(N) = N$
- ▶ N is upper bound of M
- ▶ $\sup M \leq N$



Fixed points

Kleen fixed point theorem - proof

- ▶ Lemma: if f is Scott-continuous then f is monotonic
- ▶ For any $a \leq b$:

$$f(b) = f(\sup\{a, b\}) = \sup\{f(a), f(b)\}$$

- ▶ So $f(a) \leq f(b)$

Fixed points

In context

- ▶ We care about preorder \subseteq on $\mathcal{P}(\Sigma^*)$
- ▶ For subset $D \subseteq \mathcal{P}(\Sigma^*)$:

$$\sup D = \bigcup_{d \in D} d$$

- ▶ Least element of $\mathcal{P}(\Sigma^*)$ is \emptyset

μ -Regular Expressions

Scott-continuity

- ▶ We want least fixed point of $M \mapsto L^{\sigma \cup \{X \mapsto M\}}(A)$
- ▶ So show it is Scott-continuous

μ -Regular Expressions

Scott-continuity

- ▶ We want least fixed point of $M \mapsto L^{\sigma \cup \{X \mapsto M\}}(A)$
- ▶ So show it is Scott-continuous
- ▶ By induction on A !

μ -Regular Expressions

Scott-continuity

- ▶ We want least fixed point of $M \mapsto L^{\sigma \cup \{X \mapsto M\}}(A)$
- ▶ So show it is Scott-continuous
- ▶ By induction on A !
- ▶ We need a stronger inductive hypothesis:
 - ▶ For μ -RE $A \in R_\Sigma$
 - ▶ and variable $X \in \mathcal{V}$
 - ▶ and context $\sigma : (\text{FV}(A) \setminus \{X\}) \rightarrow \mathcal{P}(\Sigma^*)$
 - ▶ Let $f_{\sigma, X, A}(M) := L^{\sigma \cup \{X \mapsto M\}}(A)$
 - ▶ Then $f_{\sigma, X, A}$ is Scott-continuous
- ▶ If σ and X are obvious, write f_A for $f_{\sigma, X, A}$

μ -Regular Expressions

Scott-continuity

► Cases:

$$A = \emptyset$$

$$f_{\emptyset}(M) = \emptyset$$

$$A = \epsilon$$

$$f_{\epsilon}(M) = \{\epsilon\}$$

$$A = x \in \Sigma$$

$$f_x(M) = \{x\}$$

$$A = Y \neq X$$

$$f_{\sigma, X, Y}(M) = \sigma(Y)$$

► f_A is constant (taking value G)

► So $f_A(\sup D) = G = \sup\{G\} = \sup(f_A[D])$ for all D

μ -Regular Expressions

Scott-continuity

- ▶ Case $A = X$:
- ▶ $f_{\sigma, X, X}(M) = L^{\sigma \cup \{X \mapsto M\}}(X) = M$

$$f_{\sigma, X, X}(\sup D) = \sup D = \sup(f_{\sigma, X, X}[D])$$

μ -Regular Expressions

Scott-continuity — Concatenation

- ▶ case $A = BC$ for μ -REs B and C
- ▶ For any directed supset D :

$$\begin{aligned} f_{BC}(\sup D) &= f_B(\sup D) f_C(\sup D) \\ &= \sup(f_B[D]) \sup(f_C[D]) \end{aligned} \tag{IH}$$

- ▶ Goal: $\sup(f_{BC}[D]) = \sup(f_B[D]) \sup(f_C[D])$
- ▶ So we need to show
 1. $\sup(f_B[D]) \sup(f_C[D])$ is an upper bound of $f_{BC}[D]$
 2. $\sup(f_B[D]) \sup(f_C[D]) \leq U$ any other upper bound U

μ -Regular Expressions

Scott-continuity — Concatenation (1)

Goal: $\sup(f_B[D]) \sup(f_C[D])$ is an upper bound of $f_{BC}[D]$

- ▶ For any $G \in f_{BC}[D]$:
- ▶ $G = f_{BC}(G')$ for some $G' \in D$
- ▶ So $G = f_B(G')f_C(G')$
- ▶ $f_B(G') \in \sup(f_B[D])$ and $f_C(G') \in \sup(f_C[D])$
- ▶ So $G \in \sup(f_B[D]) \sup(f_C[D])$

μ -Regular Expressions

Scott-continuity — Concatenation (2)

Goal: $\sup(f_B[D]) \sup(f_C[D]) \subseteq U$ for upper bound U of $f_{BC}[D]$

- ▶ For any $w \in \sup(f_B[D]) \sup(f_C[D])$
- ▶ $w = uv$ for $u \in \sup(f_B[D])$ and $v \in \sup(f_C[D])$
- ▶ So $u \in f_B(G)$ and $v \in f_C(F)$ for some $G, F \in D$
- ▶ D is directed, so exists $H \in D$ with $G, F \subseteq H$
- ▶ f_B and f_C are Scott-continuous and hence monotonic
- ▶ So $u \in f_B(H)$ and $v \in f_C(H)$
- ▶ So $w = uv \in f_{BC}(H) \subseteq U$

μ -Regular Expressions

Scott-continuity

- ▶ Case $A = B + C$ is similar to case $A = BC$
- ▶ See supplementary material for full proof (link at end)

μ -Regular Expressions

Scott-continuity – $\mu Y.B$

- ▶ Case $A = \mu Y.B$
- ▶ Goal: $f_{\sigma,X,\mu Y.B}(\sup D) = \sup(f_{\sigma,X,\mu Y.B}[D])$
- ▶ By IH, $f_{\sigma',Y,B}$ is Scott-continuous, so

$$L^{\sigma'}(\mu Y.B) = \mu(f_{\sigma',Y,B}) = \sup\{f_{\sigma',Y,B}^n(\emptyset) \mid n \in \mathbb{N}\}$$

μ -Regular Expressions

Scott-continuity – $\mu Y.B$

► Lemma: $h_n(G) := f_{\sigma \cup \{X \mapsto G\}, Y, B}^n(\emptyset)$ is Scott-continuous

$$\begin{aligned}\sup(f_{\sigma, X, \mu Y.B}[D]) &= \sup(L^{\sigma \cup \{X \mapsto G\}}(\mu Y.B) \mid G \in D) \\&= \sup\{\sup\{f_{\sigma \cup \{X \mapsto G\}, Y, B}^n(\emptyset) \mid n \in \mathbb{N}\} \mid G \in D\} \\&= \sup\{\sup\{h_n(G) \mid G \in D\} \mid n \in \mathbb{N}\} \\&= \sup\{f_{\sigma \cup \{X \mapsto \sup D\}, Y, B}^n(\emptyset) \mid n \in \mathbb{N}\} \\&= L^{\sigma \cup \{X \mapsto \sup D\}}(\mu Y.B) \\&= f_{\sigma, X, \mu Y.B}(\sup D)\end{aligned}$$

μ -Regular Expressions

Scott-continuity – $\mu Y.B$

► Lemma: $h_n(G) := f_{\sigma \cup \{X \mapsto G\}, Y, B}^n(\emptyset)$ is Scott-continuous

$$\begin{aligned}\sup(f_{\sigma, X, \mu Y.B}[D]) &= \sup(L^{\sigma \cup \{X \mapsto G\}}(\mu Y.B) \mid G \in D) \\&= \sup\{\sup\{f_{\sigma \cup \{X \mapsto G\}, Y, B}^n(\emptyset) \mid n \in \mathbb{N}\} \mid G \in D\} \\&= \sup\{\sup\{h_n(G) \mid G \in D\} \mid n \in \mathbb{N}\} \\&= \sup\{f_{\sigma \cup \{X \mapsto \sup D\}, Y, B}^n(\emptyset) \mid n \in \mathbb{N}\} \\&= L^{\sigma \cup \{X \mapsto \sup D\}}(\mu Y.B) \\&= f_{\sigma, X, \mu Y.B}(\sup D)\end{aligned}$$

μ -Regular Expressions

Scott-continuity – $\mu Y.B$

► Lemma: $h_n(G) := f_{\sigma \cup \{X \mapsto G\}, Y, B}^n(\emptyset)$ is Scott-continuous

$$\begin{aligned}\sup(f_{\sigma, X, \mu Y.B}[D]) &= \sup(L^{\sigma \cup \{X \mapsto G\}}(\mu Y.B) \mid G \in D) \\&= \sup\{\sup\{f_{\sigma \cup \{X \mapsto G\}, Y, B}^n(\emptyset) \mid n \in \mathbb{N}\} \mid G \in D\} \\&= \sup\{\sup\{h_n(G) \mid G \in D\} \mid n \in \mathbb{N}\} \\&= \sup\{f_{\sigma \cup \{X \mapsto \sup D\}, Y, B}^n(\emptyset) \mid n \in \mathbb{N}\} \\&= L^{\sigma \cup \{X \mapsto \sup D\}}(\mu Y.B) \\&= f_{\sigma, X, \mu Y.B}(\sup D)\end{aligned}$$

μ -Regular Expressions

Scott-continuity – $\mu Y.B$

► Lemma: $h_n(G) := f_{\sigma \cup \{X \mapsto G\}, Y, B}^n(\emptyset)$ is Scott-continuous

$$\begin{aligned}\sup(f_{\sigma, X, \mu Y.B}[D]) &= \sup(L^{\sigma \cup \{X \mapsto G\}}(\mu Y.B) \mid G \in D) \\&= \sup\{\sup\{f_{\sigma \cup \{X \mapsto G\}, Y, B}^n(\emptyset) \mid n \in \mathbb{N}\} \mid G \in D\} \\&= \sup\{\sup\{h_n(G) \mid G \in D\} \mid n \in \mathbb{N}\} \\&= \sup\{f_{\sigma \cup \{X \mapsto \sup D\}, Y, B}^n(\emptyset) \mid n \in \mathbb{N}\} \\&= L^{\sigma \cup \{X \mapsto \sup D\}}(\mu Y.B) \\&= f_{\sigma, X, \mu Y.B}(\sup D)\end{aligned}$$

μ -Regular Expressions

Scott-continuity – $\mu Y.B$

► Lemma: $h_n(G) := f_{\sigma \cup \{X \mapsto G\}, Y, B}^n(\emptyset)$ is Scott-continuous

$$\begin{aligned}\sup(f_{\sigma, X, \mu Y.B}[D]) &= \sup(L^{\sigma \cup \{X \mapsto G\}}(\mu Y.B) \mid G \in D) \\&= \sup\{\sup\{f_{\sigma \cup \{X \mapsto G\}, Y, B}^n(\emptyset) \mid n \in \mathbb{N}\} \mid G \in D\} \\&= \sup\{\sup\{h_n(G) \mid G \in D\} \mid n \in \mathbb{N}\} \\&= \sup\{f_{\sigma \cup \{X \mapsto \sup D\}, Y, B}^n(\emptyset) \mid n \in \mathbb{N}\} \\&= L^{\sigma \cup \{X \mapsto \sup D\}}(\mu Y.B) \\&= f_{\sigma, X, \mu Y.B}(\sup D)\end{aligned}$$

μ -Regular Expressions

Scott-continuity – $\mu Y.B$

- ▶ Lemma: $h_n(G) := f_{\sigma \cup \{X \mapsto G\}, Y, B}^n(\emptyset)$ is Scott-continuous

μ -Regular Expressions

Scott-continuity – $\mu Y.B$

- ▶ Lemma: $h_n(G) := f_{\sigma \cup \{X \mapsto G\}, Y, B}^n(\emptyset)$ is Scott-continuous
- ▶ Proof by induction on n
- ▶ Case $n = 0$:

$$h_n(G) = f_{\sigma \cup \{X \mapsto G\}, Y, B}^0(\emptyset) = \emptyset$$

μ -Regular Expressions

Scott-continuity – $\mu Y.B$

- ▶ Lemma: $h_n(G) := f_{\sigma \cup \{X \mapsto G\}, Y, B}^n(\emptyset)$ is Scott-continuous

μ -Regular Expressions

Scott-continuity – $\mu Y.B$

- ▶ Lemma: $h_n(G) := f_{\sigma \cup \{X \mapsto G\}, Y, B}^n(\emptyset)$ is Scott-continuous
- ▶ Case $n = k + 1$:
- ▶ By IH, h_k is Scott-continuous

$$N_1 := h_{k+1}[D] = \{f_{\sigma \cup \{X \mapsto G\}, Y, B}(h_k(G)) \mid G \in D\}$$

$$N_2 := \{f_{\sigma \cup \{X \mapsto G\}, Y, B}(\sup(h_k[D])) \mid G \in D\}$$

- ▶ Want to show $\sup N_1 = \sup N_2$
- ▶ Claim: N_1 and N_2 have the same upper bounds

μ -Regular Expressions

Scott-continuity – $\mu Y.B$

$$N_1 = \{f_{\sigma \cup \{X \mapsto G\}, Y, B}(h_k(G)) \mid G \in D\}$$

$$N_2 = \{f_{\sigma \cup \{X \mapsto G\}, Y, B}(\sup(h_k[D])) \mid G \in D\}$$

- ▶ Let U be an upper bound of N_1
- ▶ For all $A \in N_2$, we want $A \subseteq U$ ie $w \in A \implies w \in U$

$$\begin{aligned} A &= f_{\sigma \cup \{X \mapsto G\}, Y, B}(\sup(h_k[D])) && \text{(for some } G \in D) \\ &= \sup(f_{\sigma \cup \{X \mapsto G\}, Y, B}[h_k[D]]) \\ &= \bigcup_{F \in D} f_{\sigma \cup \{X \mapsto G\}, Y, B}(h_k(F)) \end{aligned}$$

- ▶ So $w \in f_{\sigma \cup \{X \mapsto G\}, Y, B}(h_k(F))$

μ -Regular Expressions

Scott-continuity – $\mu Y.B$

$$N_1 = \{f_{\sigma \cup \{X \mapsto G\}, Y, B}(h_k(G)) \mid G \in D\}$$

$$N_2 = \{f_{\sigma \cup \{X \mapsto G\}, Y, B}(\sup(h_k[D])) \mid G \in D\}$$

- ▶ Let U be an upper bound of N_1
- ▶ For all $A \in N_2$, we want $A \subseteq U$ ie $w \in A \implies w \in U$
- ▶ So $w \in f_{\sigma \cup \{X \mapsto G\}, Y, B}(h_k(F))$
- ▶ D directed, so there exists $H \in D$ with $G, F \subseteq H$
- ▶ $f_{\sigma', Z, B}$ and h_k Scott-continuous and hence monotonic
- ▶ So $w \in f_{\sigma \cup \{X \mapsto H\}, Y, B}(h_k(H)) \in N_1$
- ▶ Hence $w \in U$

μ -Regular Expressions

Scott-continuity – $\mu Y.B$

$$N_1 = \{f_{\sigma \cup \{X \mapsto G\}, Y, B}(h_k(G)) \mid G \in D\}$$

$$N_2 = \{f_{\sigma \cup \{X \mapsto G\}, Y, B}(\sup(h_k[D])) \mid G \in D\}$$

- ▶ Let U be an upper bound of N_1
- ▶ For all $A \in N_2$, we want $A \subseteq U$ ie $w \in A \implies w \in U$
- ▶ So $w \in f_{\sigma \cup \{X \mapsto G\}, Y, B}(h_k(F))$
- ▶ D directed, so there exists $H \in D$ with $G, F \subseteq H$
- ▶ $f_{\sigma', Z, B}$ and h_k Scott-continuous and hence monotonic
- ▶ So $w \in f_{\sigma \cup \{X \mapsto H\}, Y, B}(h_k(H)) \in N_1$
- ▶ Hence $w \in U$

μ -Regular Expressions

Scott-continuity – $\mu Y.B$

$$N_1 = \{f_{\sigma \cup \{X \mapsto G\}, Y, B}(h_k(G)) \mid G \in D\}$$

$$N_2 = \{f_{\sigma \cup \{X \mapsto G\}, Y, B}(\sup(h_k[D])) \mid G \in D\}$$

- ▶ Now the other way!
- ▶ Let U be an upper bound of N_2
- ▶ For all $A \in N_1$ we want $A \subseteq U$
- ▶ Then $A = f_{\sigma \cup \{X \mapsto G\}, Y, B}(h_k(G))$ for some $G \in D$
- ▶ $f_{\sigma \cup \{X \mapsto G\}, Y, B}$ is Scott-continuous and hence monotonic
- ▶ So $A \subseteq f_{\sigma \cup \{X \mapsto G\}, Y, B}(\sup(h_k[D])) \in N_2$
- ▶ So $A \subseteq U$

μ -Regular Expressions

Scott-continuity – $\mu Y.B$

$$N_1 = \{f_{\sigma \cup \{X \mapsto G\}, Y, B}(h_k(G)) \mid G \in D\}$$

$$N_2 = \{f_{\sigma \cup \{X \mapsto G\}, Y, B}(\sup(h_k[D])) \mid G \in D\}$$

- ▶ N_1 and N_2 have the same set of upper bounds
- ▶ So $\sup N_1 = \sup N_2$

μ -Regular Expressions

Scott-continuity – $\mu Y.B$

- We can now show that h_{k+1} is Scott-continuous

$$\begin{aligned}\sup(h_{k+1}[D]) &= \sup\{f_{\sigma \cup \{X \mapsto G\}, Y, B}(h_k(G)) \mid G \in D\} \\ &= \sup\{f_{\sigma \cup \{X \mapsto G\}, Y, B}(\sup(h_k[D])) \mid G \in D\} \\ &= \sup\{f_{\sigma \cup \{Y \mapsto \sup(h_k[D])\}, X, B}(G) \mid G \in D\} \\ &= f_{\sigma \cup \{Y \mapsto \sup(h_k[D])\}, X, B}(\sup G) \\ &= f_{\sigma \cup \{X \sup D\}, Y, B}(\sup(h_k[D])) \\ &= h_{k+1}(\sup D)\end{aligned}$$



Conclusion

- ▶ μ -Regular Expressions extend REs with a least fixed point operator
- ▶ Kleene fixed point theorem characterises this least fixed point
- ▶ Supplementary material: <https://z-snails.github.io/>